Examples/Imp/Equiv.lean
@@ -15,6 +15,14 @@ abbrev EquivOn (vars : List String) (s₁ s₂ : Stmt) : Prop :=
     BigStep st s₂ st₂' →
     st₁'.equivOn vars st₂'
 
+attribute [local grind unfold] AStmt.toStmt
+attribute [local grind unfold] State.update beval aeval
+attribute [local grind] vc pre
+attribute [local grind unfold] Assertion.entails Assertion.subst
+
+@[grind →]
+theorem valid_implies_big_step {P Q : Assertion} {st st' : State} {s : Stmt}: Valid P s Q → BigStep st s st' → P st → Q st' := by
+  grind [Valid]
 
 
 namespace Swap
@@ -42,23 +50,22 @@ def swap_spec (st : State) : State :=
 theorem swap1_meets_spec (initial : State):
   Valid (fun st => st = initial) swap1.toStmt (fun st => st.equivOn ["x", "y"] (swap_spec initial)) := by
   apply vc'_sound
-  simp [vc', Assertion.entails, swap1, Assertion.subst, aeval, State.update, swap_spec, State.equivOn]
+  simp [swap1, swap_spec]
+  grind
+
 
 theorem swap2_meets_spec (initial : State):
   Valid (fun st => st = initial) swap2.toStmt (fun st => st.equivOn ["x", "y"] (swap_spec initial)) := by
   apply vc'_sound
-  simp [vc', Assertion.entails, swap2, Assertion.subst, aeval, State.update, swap_spec, State.equivOn]
-  omega
+  simp [swap2, swap_spec]
+  grind
 
 
 theorem swap1_swap2_equiv : EquivOn ["x", "y"] swap1.toStmt swap2.toStmt := by
   simp [EquivOn]
   intros st st₁' st₂' H1 H2
-  have st1 : st₁'.equivOn ["x", "y"] (swap_spec st) := by
-    apply (swap1_meets_spec st) st st₁' (by simp) H1
-  have st2 : st₂'.equivOn ["x", "y"] (swap_spec st) := by
-    apply (swap2_meets_spec st) st st₂' (by simp) H2
-  grind
+  grind [swap1_meets_spec st, swap2_meets_spec st]
+
 
 end Swap
 
@@ -104,6 +111,10 @@ def count_up_inv := [aimp|
   }
 ]
 
+@[grind =]
+theorem count_up_inv_stmt : count_up_inv.toStmt = count_up := by
+  simp [count_up, count_up_inv, AStmt.toStmt]
+
 def count_spec (initial : State) : State :=
   let n := initial "n"
   if n < 0 then
@@ -121,25 +132,15 @@ def count_end_state : Assertion := fun st =>
     sum == (n * (n + 1)) / 2
 
 
+
+@[grind →]
+theorem squish_up (a b : Int): a ≤ b + 1 ∧ b < a → a = b + 1 := by omega
+
+
 theorem count_up_to_end_state : Valid (fun _ => True) count_up_inv.toStmt count_end_state := by
   apply vc'_sound
-  simp [vc', Assertion.entails, count_up_inv, Assertion.subst, aeval, State.update, count_end_state]
-  simp [inv_up, beval, aeval, State.update]
-  constructor
-  · constructor
-    · intros st h1 h2
-      grind
-    · intros s h1 h2
-      cases h1
-      · simp_all
-      · have : s "n" >= 0 := by omega
-        split
-        · omega
-        · have : s "i" = s "n" + 1 := by omega
-          simp_all
-          grind
-  · omega
-
+  simp [count_up_inv, count_end_state]
+  grind [Int.mul_comm, inv_up]
 
 
 def inv_down: Assertion := fun st =>
@@ -159,23 +160,18 @@ def count_down_inv := [aimp|
   }
 ]
 
+@[grind =]
+theorem count_down_inv_stmt : count_down_inv.toStmt = count_down := by
+  simp [count_down, count_down_inv, AStmt.toStmt]
+
+@[grind →]
+theorem squish_down (a b : Int) : a < (b + 1) → b ≤ a → a = b := by omega
+
+
 theorem count_down_to_end_state : Valid (fun _ => True) count_down_inv.toStmt count_end_state := by
   apply vc'_sound
-  simp [vc', Assertion.entails, count_down_inv, Assertion.subst, aeval, State.update, count_end_state]
-  simp [inv_down, beval, aeval, State.update]
-  constructor
-  · constructor
-    · intros st h1 h2
-      grind
-    · intros s h1 h2
-      cases h1
-      · simp_all
-      · have : s "n" >= 0 := by omega
-        split
-        · omega
-        · have : s "i" = -1 := by omega
-          simp_all
-  · omega
+  simp [count_down_inv, count_end_state]
+  grind [inv_down]
 
 
 def inv_n_eq (k : Int) : Assertion := fun st => st "n" = k
@@ -189,6 +185,11 @@ def count_up_n_inv (k : Int) := [aimp|
   }
 ]
 
+@[grind =]
+theorem count_up_n_inv_stmt (k : Int) : (count_up_n_inv k).toStmt = count_up := by
+  simp [count_up, count_up_n_inv, AStmt.toStmt]
+
+
 def count_down_n_inv (k : Int) := [aimp|
   sum := 0;
   i := n;
@@ -198,37 +199,44 @@ def count_down_n_inv (k : Int) := [aimp|
   }
 ]
 
-theorem count_up_preserves_n (k : Int) :
-    Valid (fun st => st "n" = k) count_up_inv.toStmt (fun st' => st' "n" = k) := by
-  show Valid (fun st => st "n" = k) (count_up_n_inv k).toStmt (inv_n_eq k)
+@[grind =]
+theorem count_down_n_inv_stmt (k : Int) : (count_down_n_inv k).toStmt = count_down := by
+  simp [count_down, count_down_n_inv, AStmt.toStmt]
+
+theorem count_up_preserves_n_triple (k : Int) :
+  Valid (fun st => st "n" = k) (count_up_n_inv k).toStmt (inv_n_eq k) := by
   apply vc'_sound
-  simp [vc', count_up_n_inv, vc, inv_n_eq, Assertion.subst, aeval, State.update,
-        beval, pre, Assertion.entails]
-  constructor <;> intro st h _ <;> exact h
+  simp [count_up_n_inv]
+  grind [inv_n_eq]
 
-theorem count_down_preserves_n (k : Int) :
-    Valid (fun st => st "n" = k) count_down_inv.toStmt (fun st' => st' "n" = k) := by
-  show Valid (fun st => st "n" = k) (count_down_n_inv k).toStmt (inv_n_eq k)
+
+@[grind →]
+theorem count_up_preserves_n (st st' : State) :
+  BigStep st count_up st' → st "n" = st' "n" := by
+  intros h
+  have h' := count_up_preserves_n_triple (st "n")
+  have h'' := valid_implies_big_step h' h
+  grind [inv_n_eq, count_up_n_inv]
+
+
+
+theorem count_down_preserves_n_triple (k : Int) :
+    Valid (fun st => st "n" = k) (count_down_n_inv k).toStmt (inv_n_eq k) := by
   apply vc'_sound
-  simp [vc', count_down_n_inv, vc, inv_n_eq, Assertion.subst, aeval, State.update,
-        beval, pre, Assertion.entails]
-  constructor <;> intro st h _ <;> exact h
+  simp [count_down_n_inv]
+  grind [inv_n_eq]
 
-theorem count_up_down_equiv : EquivOn ["sum"] count_up_inv.toStmt count_down_inv.toStmt := by
-  simp [EquivOn, State.equivOn]
-  intros st st₁' st₂' H1 H2
-  have ce1 := count_up_to_end_state st st₁' trivial H1
-  have ce2 := count_down_to_end_state st st₂' trivial H2
-  have hn1 : st₁' "n" = st "n" := count_up_preserves_n (st "n") st st₁' rfl H1
-  have hn2 : st₂' "n" = st "n" := count_down_preserves_n (st "n") st st₂' rfl H2
-  simp only [count_end_state] at ce1 ce2
-  rw [hn1] at ce1
-  rw [hn2] at ce2
-  split at ce1 <;> simp_all <;> omega
 
+@[grind →]
+theorem count_down_preserves_n (st st' : State) :
+  BigStep st count_down st' → st "n" = st' "n" := by
+  have := count_down_preserves_n_triple (st "n")
+  grind [inv_n_eq, count_down_n_inv]
+
+
+theorem count_up_down_equiv : EquivOn ["sum"] count_up count_down := by
+  grind [count_end_state, count_up_to_end_state, count_down_to_end_state]
 
 
 end Count
-
-
 end Imp
